Incorporating Peter Lammich's suggestions

WebAssembly/Wasm_Instantiation_Monad_Properties.thy
@@ -1,66 +1,73 @@
 theory Wasm_Instantiation_Monad_Properties 
   imports "../libs/Misc_Generic_Lemmas" "../libs/List_Assn" 
-    Wasm_Instantiation_Monad Wasm_Monad_Assertions Wasm_Instantiation_Properties begin
+    Wasm_Instantiation_Monad Wasm_Monad_Assertions Wasm_Instantiation_Properties     
+    
+    
+begin
 
+lemma list_blit_array_triple:
+  "<a \<mapsto>\<^sub>a la> 
+  list_blit_array l a n
+  <\<lambda>r. \<up>(fits_at_in l n la) 
+    * a \<mapsto>\<^sub>a insert_at_in l n la>"
+proof(induct l arbitrary:a la n)
+case Nil
+  then show ?case by sep_auto
+next
+  case (Cons a l)
+  show ?case 
+    supply [simp del] = list_blit_array.simps
+    apply(subst list_blit_array.simps)
+    apply(sep_auto heap:Cons split:list.splits simp: take_update_last)
+    done
+qed
 
-lemma fold_map_triple:
-  assumes "\<And> x. <F> f x <\<lambda>r. Q x r * F>"
-  shows "<F> 
-  Heap_Monad.fold_map f xs 
-  <\<lambda>r. list_assn Q xs r * F>"
-  using assms 
-proof(induct xs)
+lemma fold_map_decon:
+  assumes "\<And> x. <P> f x <\<lambda>r. Q x r * P>"
+  assumes "\<And>ys. list_assn Q xs ys * P \<Longrightarrow>\<^sub>A Q' ys"
+  shows 
+    "<P> Heap_Monad.fold_map f xs <Q'>"
+  using assms
+proof(induct xs arbitrary:P Q')
   case Nil
   then show ?case by sep_auto
 next
   case (Cons a xs)
-  show ?case 
-    by (sep_auto heap:Cons(2) Cons(1)[OF Cons(2)])
-qed
-
-
-lemma array_blit_map_triple:
-  assumes  "\<And> x. <F> f x <\<lambda>r. Q x r * F>"
-  shows 
-    "<a \<mapsto>\<^sub>a la * F> 
-    array_blit_map xs f a n
-    <\<lambda>r. \<exists>\<^sub>Ays. \<up>(fits_at_in xs n la)
-  *  a \<mapsto>\<^sub>a insert_at_in ys n la
-  * list_assn Q xs ys * F>"
-proof -
   {
-    fix ys
-    have "<a \<mapsto>\<^sub>a la * list_assn Q xs ys * F> 
-    list_blit_array ys a n
-    <\<lambda>r.\<up>(fits_at_in xs n la)
-  *  a \<mapsto>\<^sub>a insert_at_in ys n la 
-  * list_assn Q xs ys * F>"
-      supply [simp del] = list_blit_array.simps
-      apply(extract_pre_pure)
-      apply(sep_auto heap: list_blit_array_triple split:list.splits)
-      done
+    fix y ys
+    have "list_assn Q xs ys * ( Q a y * P) \<Longrightarrow>\<^sub>A  Q' (y#ys)" using Cons(3)[of "y#ys"] 
+      by (simp add: assn_times_assoc star_aci(3))
   }
   note 1 = this
+  show ?case  
+    apply(sep_auto heap:Cons(2) Cons(1)[OF Cons(2)])
+    using 1 star_aci(2) star_aci(3) by auto
+qed
 
-  show ?thesis 
-    supply [simp del] = list_blit_array.simps
-    apply(sep_auto heap:fold_map_triple[OF assms] 1) 
-    done 
-qed 
-
-lemma array_blit_map_triple_emp:
-  assumes  "\<And> x. <emp> f x <\<lambda>r. Q x r>"
+lemma array_blit_map_decon:
+  assumes "P \<Longrightarrow>\<^sub>A a \<mapsto>\<^sub>a la * F"
+  assumes "\<And> x. <F> f x <\<lambda>r. Q x r * F>"
+  assumes "\<And>ys. fits_at_in xs n la \<Longrightarrow> 
+    a \<mapsto>\<^sub>a insert_at_in ys n la * list_assn Q xs ys * F \<Longrightarrow>\<^sub>A Q' ()"
   shows 
-    "<a \<mapsto>\<^sub>a la> 
+    "<P> 
     array_blit_map xs f a n
-    <\<lambda>r. \<exists>\<^sub>Ays. \<up>(fits_at_in xs n la)
-  *  a \<mapsto>\<^sub>a insert_at_in ys n la
-  * list_assn Q xs ys>"
-  using array_blit_map_triple[of emp f Q a la xs n]
-  by(simp del:array_blit_map.simps add:assms) 
+    <Q'>"
+  supply [simp del] = Heap_Monad.fold_map.simps list_blit_array.simps
+  apply (rule cons_pre_rule[OF assms(1)])  
+  apply (sep_auto)
+   apply (vcg heap:fold_map_decon[OF assms(2)])
+   apply(solve_entails)
+  apply(extract_pre_pure)
+  apply(sep_auto heap:list_blit_array_triple)
+  subgoal using assms(3) by auto
+  by (metis assms(3))
 
 abbreviation "module_func_to_cl inst inst_types \<equiv> 
   (\<lambda>(i_t, loc_ts, b_es). cl.Func_native inst (inst_types!i_t) loc_ts b_es)"
+
+abbreviation "module_func_to_cl_m inst_m inst_types \<equiv> 
+  (\<lambda>(i_t, loc_ts, b_es). cl_m.Func_native inst_m (inst_types!i_t) loc_ts b_es)"
 
 abbreviation "alloc_funcs_simple' m_fs inst inst_types \<equiv> 
   map (\<lambda>m_f. module_func_to_cl inst inst_types m_f) m_fs" 
@@ -74,7 +81,7 @@ lemma list_assn_map1:"list_assn P (map f xs) ys = list_assn (\<lambda>x y. P (f 
 
 lemma list_assn_pure:"list_assn (\<lambda>x y. \<up>(P x y)) xs ys = \<up>(list_all2 P xs ys)"
   by(induct "\<lambda>x y. \<up>(P x y)"  xs ys rule: list_assn.induct, auto)
-  
+
 lemma alloc_funcs_m_triple:
   "< s_funcs \<mapsto>\<^sub>a fs * inst_types \<mapsto>\<^sub>a m_tfs> 
   alloc_funcs_m s_funcs n m_fs inst_m inst_types
@@ -82,11 +89,15 @@ lemma alloc_funcs_m_triple:
   *  s_funcs \<mapsto>\<^sub>a insert_at_in ys n fs
   *  \<up>(list_all2 (cl_m_agree ([inst], [inst_m])) (alloc_funcs_simple' m_fs inst m_tfs) ys)
   *  inst_types \<mapsto>\<^sub>a m_tfs>"
-  unfolding alloc_funcs_m_def cl_m_agree_j_def
-  apply(simp only: list_all2_map1 flip:list_assn_pure)
-  apply(rule array_blit_map_triple) 
-  apply(sep_auto)
-  done
+  unfolding alloc_funcs_m_def 
+  supply [simp del] = array_blit_map.simps
+  apply(vcg 
+      decon:array_blit_map_decon[where Q="\<lambda>m_f r. \<up>(r = module_func_to_cl_m inst_m m_tfs m_f)"])
+    apply(solve_entails)
+   apply(sep_auto)
+  apply(sep_auto simp:list_assn_pure)
+  by(simp add: list_all2_map1 list_all2_conv_all_nth cl_m_agree_j_def split:prod.splits)
+
 
 lemma alloc_tabs_m_triple: 
   "< s_tabs \<mapsto>\<^sub>a ts> 
@@ -94,8 +105,15 @@ lemma alloc_tabs_m_triple:
   <\<lambda>r.\<exists>\<^sub>Ays. \<up>(fits_at_in m_ts n ts)
   *  s_tabs \<mapsto>\<^sub>a insert_at_in ys n ts
   *  list_assn tabinst_m_assn (alloc_tabs_simple m_ts) ys>"
-  unfolding alloc_tabs_m_def tabinst_m_assn_def alloc_tab_simple_def
-  by(simp only: list_assn_map1, rule array_blit_map_triple_emp, sep_auto)
+  unfolding alloc_tabs_m_def 
+  supply [simp del] = array_blit_map.simps
+  apply(vcg decon: array_blit_map_decon
+      [where F=emp and Q="\<lambda>tt t_m. tabinst_m_assn (alloc_tab_simple tt) t_m"])
+    apply solve_entails
+   apply (sep_auto simp:tabinst_m_assn_def alloc_tab_simple_def)
+  apply (sep_auto simp:list_assn_map1)
+  done
+
 
 lemma alloc_mems_m_triple: 
   "< s_mems \<mapsto>\<^sub>a ms> 
@@ -103,27 +121,36 @@ lemma alloc_mems_m_triple:
   <\<lambda>r.\<exists>\<^sub>Ays. \<up>(fits_at_in m_ms n ms)
   *  s_mems \<mapsto>\<^sub>a insert_at_in ys n ms
   *  list_assn mem_m_assn (alloc_mems_simple m_ms) ys>"
-  unfolding alloc_mems_m_def mem_m_assn_def alloc_mem_simple_def
-  apply(simp only: list_assn_map1, rule array_blit_map_triple_emp)
-  apply(sep_auto simp:mem_mk_def mem_rep_mk_def bytes_replicate_def 
-      zero_byte_def mem_rep.Abs_mem_rep_inverse)
+  unfolding alloc_mems_m_def
+  supply [simp del] = array_blit_map.simps
+  apply(vcg decon: array_blit_map_decon
+      [where F=emp and Q="\<lambda>mt m_m. mem_m_assn (alloc_mem_simple mt) m_m"])
+    apply(solve_entails)
+   apply(sep_auto)
+   apply(sep_auto simp:mem_m_assn_def alloc_mem_simple_def mem_mk_def mem_rep_mk_def 
+      bytes_replicate_def zero_byte_def mem_rep.Abs_mem_rep_inverse)
+  apply(sep_auto simp:list_assn_map1)
   done
 
+lemma list_all2_eq_map_conv:"(list_all2 (\<lambda>x y. f x = g y) xs ys) = (map f xs = map g ys)"
+  unfolding list_all2_conv_all_nth
+  by (metis length_map map_intro_length nth_map)
 
 (* todo: learn how to make this nicer *)
 lemma alloc_globs_m_triple': 
   "< s_globs \<mapsto>\<^sub>a gs> 
   alloc_globs_m s_globs n m_gs gvs 
-  <\<lambda>r.\<exists>\<^sub>Ays. \<up>(fits_at_in (zip m_gs gvs) n gs)
-  *  s_globs \<mapsto>\<^sub>a insert_at_in ys n gs
-  *  \<up>((alloc_globs_simple m_gs gvs) = ys)>"
-  unfolding alloc_globs_m_def alloc_glob_simple_def
-  apply(simp only: list.rel_eq list_assn_pure flip: list.rel_eq list_assn_pure)
-  apply(simp only: list_assn_map1)
-  apply(rule array_blit_map_triple_emp)
-  apply(sep_auto)
+  <\<lambda>r.\<up>(fits_at_in (zip m_gs gvs) n gs)
+  *  s_globs \<mapsto>\<^sub>a insert_at_in (alloc_globs_simple m_gs gvs) n gs>"
+  unfolding alloc_globs_m_def 
+  supply [simp del] = array_blit_map.simps
+  apply(vcg decon: array_blit_map_decon
+      [where F=emp and Q="\<lambda>m_g_v g_m. \<up>(alloc_glob_simple m_g_v = g_m)"])
+    apply(solve_entails)
+   apply(sep_auto simp:alloc_glob_simple_def)
+  apply(sep_auto simp:list_assn_pure)
+  apply(simp add:list_all2_eq_map_conv)
   done
-
 
 lemma alloc_globs_m_triple: 
   "< s_globs \<mapsto>\<^sub>a gs> 
@@ -136,16 +163,17 @@ abbreviation "get_exports inst m_exps \<equiv>
   map (\<lambda>m_exp. \<lparr>E_name=(E_name m_exp), E_desc=(export_get_v_ext inst (E_desc m_exp))\<rparr>) m_exps"
 
 lemma get_exports_m_triple: 
-  "<f_m \<mapsto>\<^sub>a f * t_m \<mapsto>\<^sub>a t  * m_m \<mapsto>\<^sub>a m * g_m \<mapsto>\<^sub>a g> 
-  get_exports_m \<lparr>inst_m.types = tf_m, funcs = f_m, tabs = t_m, mems = m_m, globs = g_m \<rparr> m_exps 
-  <\<lambda>r. \<up>(get_exports \<lparr>inst.types = tf, funcs = f, tabs = t, mems = m, globs = g \<rparr> m_exps = r)
-  *  (f_m \<mapsto>\<^sub>a f * t_m \<mapsto>\<^sub>a t * m_m \<mapsto>\<^sub>a m * g_m \<mapsto>\<^sub>a g)>"
+  "<inst_m_assn inst inst_m> 
+  get_exports_m inst_m m_exps 
+  <\<lambda>r. \<up>(r = get_exports inst m_exps) * inst_m_assn inst inst_m>"
   unfolding get_exports_m_def 
-  apply(simp only: list.rel_eq list_assn_pure flip: list.rel_eq list_assn_pure)
-  apply(simp only: list_assn_map1)
-  apply(rule fold_map_triple)
-  unfolding export_get_v_ext_m_def export_get_v_ext_def
-  by(sep_auto split:v_ext.splits)
+  supply [simp del] = Heap_Monad.fold_map.simps
+  apply(vcg decon del:sep_decon_rules decon:fold_map_decon[where Q=
+        "\<lambda>m_exp r. \<up>(\<lparr>E_name = E_name m_exp, E_desc = export_get_v_ext inst (E_desc m_exp)\<rparr> = r)"])
+   apply(sep_auto simp:export_get_v_ext_m_def export_get_v_ext_def 
+      inst_m_assn_def split:v_ext.splits)
+  apply(sep_auto simp:list_assn_pure list_all2_eq_map_conv)
+  done
 
 lemma alloc_funcs_equiv_full:"alloc_funcs s m_fs i
   = (s\<lparr>s.funcs := s.funcs s @ alloc_funcs_simple m_fs i\<rparr>, 
@@ -228,7 +256,11 @@ proof -
    apply(sep_auto heap:alloc_tabs_m_triple)
    apply(sep_auto heap:alloc_mems_m_triple)
    apply(sep_auto heap:alloc_globs_m_triple)
-  apply(sep_auto, sep_auto heap:get_exports_m_triple)
+    (*todo: find a nicer way of splitting the get_exports_m_triple *)
+  apply(sep_auto, sep_auto heap: get_exports_m_triple
+    [of "\<lparr>inst.types = _, funcs = _, tabs = _, mems = _ , globs = _ \<rparr>"
+      "\<lparr>inst_m.types = _, funcs = _, tabs = _, mems = _ , globs = _ \<rparr>", 
+      simplified inst_m_assn_def inst.simps inst_m.simps])
   apply(extract_pre_pure)
     (* todo: find a better way of extracting length information from the hypotheses *)
   apply(subst (asm) (1) list_all2_extract_length)  
